Add CMHI vector comparison to ARM model

arm/proofs/simulator_iclasses.ml
@@ -122,6 +122,9 @@ let iclasses =
   (*** BIT ***)
   "0x101110101xxxxx000111xxxxxxxxxx";
 
+  (*** CMHI, vector ***)
+  "0x101110xx1xxxxx001101xxxxxxxxxx";
+
   (*** CNT, bias to defined size = 0 ***)
   "0x00111000100000010110xxxxxxxxxx";
   "0x001110xx100000010110xxxxxxxxxx";
