arm/proofs/instruction.ml
@@ -11,7 +11,7 @@
  *** This is used to describe the safety property of assembly programs such as
  *** the constant-time property.
  *** We define that an instruction raises an observable microarchitectural
- *** event if its cycles/power consumption/anything that can be observed by 
+ *** event if its cycles/power consumption/anything that can be observed by
  *** a side-channel attacker can vary depending on the inputs of
  *** the instruction. For example, instructions taking a constant number of
  *** cycles like ADD do not raise an observable event, whereas cond branch does.
@@ -815,6 +815,13 @@ let MAYCHANGE_REGS_AND_FLAGS_PERMITTED_BY_ABI = REWRITE_RULE
     MAYCHANGE MODIFIABLE_UPPER_SIMD_REGS ,, MAYCHANGE SOME_FLAGS ,, MAYCHANGE [events]`);;
 
 (* ------------------------------------------------------------------------- *)
+(* Mask-creating version of a comparison-type operation.                     *)
+(* ------------------------------------------------------------------------- *)
+
+let masking = new_definition
+ `(masking p:N word->N word->N word) x y = word_neg(word(bitval(p x y)))`;;
+
+(* ------------------------------------------------------------------------- *)
 (* General register-register instructions.                                   *)
 (* ------------------------------------------------------------------------- *)
 
@@ -1058,6 +1065,27 @@ let arm_CCMP = define
 let arm_CLZ = define
  `arm_CLZ Rd Rn =
         \s. (Rd := (word(word_clz (read Rn s:N word)):N word)) s`;;
+
+let arm_CMHI_VEC = define
+ `arm_CMHI_VEC Rd Rn Rm esize datasize =
+    \s:armstate.
+        let n = read Rn s in
+        let m = read Rm s in
+        if datasize = 128 then
+          let d:(128)word =
+            if esize = 64 then simd2 (masking word_ugt) n m
+            else if esize = 32 then simd4 (masking word_ugt) n m
+            else if esize = 16 then simd8 (masking word_ugt) n m
+            else simd16 (masking word_ugt) n m in
+          (Rd := d) s
+        else
+          let n:(64)word = word_subword n (0,64) in
+          let m:(64)word = word_subword m (0,64) in
+          let d:(64)word =
+            if esize = 32 then simd2 (masking word_ugt) n m
+            else if esize = 16 then simd4 (masking word_ugt) n m
+            else simd8 (masking word_ugt) n m in
+          (Rd := word_zx d:(128)word) s`;;
 
 let arm_CNT = define
  `arm_CNT Rd Rn datasize =
@@ -3004,7 +3032,8 @@ let WORD_DUPLICATE_64_128 = prove
   REWRITE_TAC[WORD_DUPLICATE_REFL]);;
 
 let all_simd_rules =
-   [usimd16;usimd8;usimd4;usimd2;simd16;simd8;simd4;simd2;o_THM;
+   [usimd16;usimd8;usimd4;usimd2;simd16;simd8;simd4;simd2;
+    o_THM; masking;
     WORD_DUPLICATE_64_128;
     word_interleave16;
     word_interleave8;word_interleave4;word_interleave2;word_split_lohi;
@@ -3019,6 +3048,7 @@ let EXPAND_SIMD_RULE =
   CONV_RULE (DEPTH_CONV DIMINDEX_CONV) o REWRITE_RULE all_simd_rules;;
 
 let arm_ADD_VEC_ALT =    EXPAND_SIMD_RULE arm_ADD_VEC;;
+let arm_CMHI_VEC_ALT =   EXPAND_SIMD_RULE arm_CMHI_VEC;;
 let arm_CNT_ALT =        EXPAND_SIMD_RULE arm_CNT;;
 let arm_DUP_GEN_ALT =    EXPAND_SIMD_RULE arm_DUP_GEN;;
 let arm_MLS_VEC_ALT =    EXPAND_SIMD_RULE arm_MLS_VEC;;
@@ -3092,7 +3122,8 @@ let ARM_OPERATION_CLAUSES =
        arm_AND; arm_AND_VEC; arm_ANDS; arm_ASR; arm_ASRV;
        arm_B; arm_BCAX; arm_BFM; arm_BIC; arm_BIC_VEC; arm_BICS; arm_BIT;
        arm_BL; arm_BL_ABSOLUTE; arm_Bcond;
-       arm_CBNZ_ALT; arm_CBZ_ALT; arm_CCMN; arm_CCMP; arm_CLZ; arm_CNT_ALT;
+       arm_CBNZ_ALT; arm_CBZ_ALT; arm_CCMN; arm_CCMP; arm_CLZ;
+       arm_CMHI_VEC_ALT; arm_CNT_ALT;
        arm_CSEL; arm_CSINC; arm_CSINV; arm_CSNEG;
        arm_DUP_GEN_ALT;
        arm_EON; arm_EOR; arm_EOR_VEC; arm_EOR3; arm_EXT; arm_EXTR;
