arm/proofs/decode.ml
@@ -371,6 +371,13 @@ let decode = new_definition `!w:int32. decode w =
     // BIC
     SOME (arm_BIC_VEC (QREG' Rd) (QREG' Rn) (QREG' Rm) (if q then 128 else 64))
 
+  | [0:1; q; 0b101110:6; size:2; 1:1; Rm:5; 0b001101:6; Rn:5; Rd:5] ->
+    // CMHI
+    if size = word 0b11 /\ ~q then NONE else
+    let esize = 8 * 2 EXP val size in
+    let datasize = if q then 128 else 64 in
+    SOME (arm_CMHI_VEC (QREG' Rd) (QREG' Rn) (QREG' Rm) esize datasize)
+
   | [0:1; q; 0b101110001:9; Rm:5; 0b000111:6; Rn:5; Rd:5] ->
     // EOR
     SOME (arm_EOR_VEC (QREG' Rd) (QREG' Rn) (QREG' Rm) (if q then 128 else 64))
